theories/case_studies/cmdc/cmdc.v
@@ -74,8 +74,7 @@ Section CMDC_Main.
 
   Definition cmdc_main_data : list Word := [WInt 0; WInt 0].
 
-  Definition cmdc_main_imports `{switcherLayout}
-    (b_assert e_assert : Addr)
+  Definition cmdc_main_imports `{!switcherLayout} `{!assertLayout}
     (B_f C_g : Sealable) : list Word :=
     [
       WSentry XSRW_ Local b_switcher e_switcher a_switcher_call;
