theories/case_studies/vae/vae_spec.v
@@ -14,7 +14,7 @@ Section VAE.
     {nainv: logrel_na_invs Σ}
     {cstackg : CSTACKG Σ}
     `{MP: MachineParameters}
-    {swlayout : switcherLayout} {swlayoutWf : switcherLayoutWf}
+    {swlayout : switcherLayout} {swlayoutWf : switcherLayoutWf} {assertlayout : assertLayout}
   .
 
   Context {C : CmptName}.
@@ -32,7 +32,6 @@ Section VAE.
 
     (b_vae_exp_tbl e_vae_exp_tbl : Addr)
 
-    (b_assert e_assert : Addr) (a_flag : Addr)
     (C_f : Sealable)
 
     (W0 : WORLD)
@@ -46,7 +45,7 @@ Section VAE.
     (i : positive)
     :
 
-    let imports := vae_main_imports b_assert e_assert C_f in
+    let imports := vae_main_imports C_f in
 
     Nswitcher ## Nassert ->
     Nswitcher ## Nvae_code ->
